chore: bump lean4 dep to leanprover/lean4:nightly-2021-08-18

deps/smtlib/src/SmtLib/Denote/Array.lean
@@ -8,7 +8,7 @@ import Galois.Data.List
 import Galois.Init.Order
 
 namespace Smt
-universes u v
+universe u v
 
 /- A finite representation of a map/array, with a set of entries
     stored in a association list and a default value to return
@@ -41,21 +41,21 @@ def FiniteMap.decEq
 instance [DecidableEq α] [DecidableEq β] : DecidableEq (FiniteMap α β) :=
   FiniteMap.decEq
 
-def FiniteMap.less [HasLess α] [HasLess β] : FiniteMap α β → FiniteMap α β → Prop
+def FiniteMap.less [LT α] [LT β] : FiniteMap α β → FiniteMap α β → Prop
   | a1, a2 => (a1.entries, a1.default) < (a2.entries, a2.default)
 
 protected
-instance FiniteMap.HasLess [HasLess α] [HasLess β] : HasLess (FiniteMap α β) :=
+instance FiniteMap.LT [LT α] [LT β] : LT (FiniteMap α β) :=
   ⟨@FiniteMap.less α β _ _⟩
 
 
 def FiniteMap.decLt
   [DecidableEq α]
   [DecidableEq β]
-  [HasLess α]
-  [HasLess β]
-  [DecidableLess α]
-  [DecidableLess β]
+  [LT α]
+  [LT β]
+  [DecidableLT α]
+  [DecidableLT β]
   : ∀ (fm1 fm2 : FiniteMap α β),
     Decidable (fm1 < fm2)
   | ⟨es1, d1⟩, ⟨es2, d2⟩ =>
@@ -64,13 +64,13 @@ def FiniteMap.decLt
     inferInstanceAs (Decidable ((es1, d1) < (es2, d2)))
 
 
-instance FiniteMap.DecidableLess
+instance FiniteMap.DecidableLT
   [DecidableEq α]
   [DecidableEq β]
-  [HasLess α]
-  [HasLess β]
-  [DecidableLess α]
-  [DecidableLess β]
+  [LT α]
+  [LT β]
+  [DecidableLT α]
+  [DecidableLT β]
   : ∀ (x y : FiniteMap α β), Decidable (x < y) :=
   FiniteMap.decLt
 
@@ -78,8 +78,8 @@ instance FiniteMap.DecidableLess
 end
 
 -- FIXME prove when tactics are enabled
-theorem HasLess.transitivity {α : Type u} {β : Type v}
- [HasLess α] [HasLess β]
+theorem LT.transitivity {α : Type u} {β : Type v}
+ [LT α] [LT β]
  [DecidableEq α] [DecidableEq β] :
  (∀ (x y z : α), x < y → y < z → x < z) →
  (∀ (x y z : β), x < y → y < z → x < z) →
@@ -87,8 +87,8 @@ theorem HasLess.transitivity {α : Type u} {β : Type v}
  sorry
 
 -- FIXME prove when tactics are enabled
-theorem HasLess.asymmetry {α : Type u} {β : Type v}
- [HasLess α] [HasLess β]
+theorem LT.asymmetry {α : Type u} {β : Type v}
+ [LT α] [LT β]
  [DecidableEq α] [DecidableEq β] :
  (∀ (x y : α), x < y → ¬(y < x)) →
  (∀ (x y : β), x < y → ¬(y < x)) →
@@ -96,8 +96,8 @@ theorem HasLess.asymmetry {α : Type u} {β : Type v}
  sorry
 
 -- FIXME prove when tactics are enabled
-theorem HasLess.totality {α : Type u} {β : Type v}
- [HasLess α] [HasLess β]
+theorem LT.totality {α : Type u} {β : Type v}
+ [LT α] [LT β]
  [DecidableEq α] [DecidableEq β] :
  (∀ (x y : α), x < y ∨ x = y ∨ y < x) →
  (∀ (x y : β), x < y ∨ x = y ∨ y < x) →
@@ -106,27 +106,27 @@ theorem HasLess.totality {α : Type u} {β : Type v}
 
 instance {α : Type u} {β : Type v}
   [DecidableEq α] [DecidableEq β]
-  [HasLess α] [HasLess β]
-  [hA : LessOrder α] [hB : LessOrder β]
-  : LessOrder (FiniteMap α β) :=
+  [LT α] [LT β]
+  [hA : LTOrder α] [hB : LTOrder β]
+  : LTOrder (FiniteMap α β) :=
   -- FIXME why don't these definitions work...?
-  { transitive := sorry, --FiniteMap.Less.transitivity hA.transitive hB.transitive,
-    asymmetric := sorry, --FiniteMap.Less.asymmetry hA.asymmetric hB.asymmetric,
-    total := sorry --FiniteMap.Less.totality hA.total hB.total
+  { transitive := sorry, --FiniteMap.LT.transitivity hA.transitive hB.transitive,
+    asymmetric := sorry, --FiniteMap.LT.asymmetry hA.asymmetric hB.asymmetric,
+    total := sorry --FiniteMap.LT.totality hA.total hB.total
   }
 
 /-- A well-formed FiniteMap has sorted entries and no default values
    stored in it's association list, which means Lean definitional equality
    corresponds to extensional equality for arrays. -/
 structure WellFormed {α : Type u} {β : Type v} (fm : FiniteMap α β)
-  [DecidableLessOrder α]
-  [DecidableLessOrder β] : Prop :=
+  [DecidableLTOrder α]
+  [DecidableLTOrder β] : Prop :=
   (sorted : fm.entries.SortedMap)
   (noDefault : fm.entries.Forall (λ (kv : α × β) => kv.snd ≠ fm.default))
 
 def empty.wellFormed (α : Type u) {β : Type v}
-  [DecidableLessOrder α]
-  [DecidableLessOrder β]
+  [DecidableLTOrder α]
+  [DecidableLTOrder β]
   (v : β) : FiniteMap.WellFormed (FiniteMap.empty α v) :=
   let hSM : List.SortedMap (FiniteMap.empty α v).entries := @List.SortedMap.nil α β _;
   ⟨hSM, List.Forall.nil⟩
@@ -137,8 +137,8 @@ end FiniteMap
 /-- An Array is simply a FiniteMap with a unique representation (imposed by
     the well-formedness requirement). -/
 def Array (α : Type u) (β : Type v)
-  [DecidableLessOrder α]
-  [DecidableLessOrder β] : Type (max u v) :=
+  [DecidableLTOrder α]
+  [DecidableLTOrder β] : Type (max u v) :=
 {fm : FiniteMap α β // FiniteMap.WellFormed fm}
 
 -- #check Subtype.Inhabited
@@ -148,26 +148,26 @@ variable {α : Type u} {β : Type v}
 
 open Subtype
 
-instance [hA : DecidableLessOrder α] [hB : DecidableLessOrder β] : DecidableEq (Array α β) :=
+instance [hA : DecidableLTOrder α] [hB : DecidableLTOrder β] : DecidableEq (Array α β) :=
   inferInstanceAs (DecidableEq {fm : FiniteMap α β // FiniteMap.WellFormed fm})
 
-instance [hA : DecidableLessOrder α] [hB : DecidableLessOrder β] : HasLess (Array α β) :=
-  inferInstanceAs (HasLess {fm : FiniteMap α β // FiniteMap.WellFormed fm})
+instance [hA : DecidableLTOrder α] [hB : DecidableLTOrder β] : LT (Array α β) :=
+  inferInstanceAs (LT {fm : FiniteMap α β // FiniteMap.WellFormed fm})
 
-instance [hA : DecidableLessOrder α] [hB : DecidableLessOrder β] : DecidableLess (Array α β) :=
-  inferInstanceAs (DecidableLess {fm : FiniteMap α β // FiniteMap.WellFormed fm})
+instance [hA : DecidableLTOrder α] [hB : DecidableLTOrder β] : DecidableLT (Array α β) :=
+  inferInstanceAs (DecidableLT {fm : FiniteMap α β // FiniteMap.WellFormed fm})
 
-instance [hA : DecidableLessOrder α] [hB : DecidableLessOrder β] : LessOrder (Array α β) :=
-  inferInstanceAs (LessOrder {fm : FiniteMap α β // FiniteMap.WellFormed fm})
+instance [hA : DecidableLTOrder α] [hB : DecidableLTOrder β] : LTOrder (Array α β) :=
+  inferInstanceAs (LTOrder {fm : FiniteMap α β // FiniteMap.WellFormed fm})
 
-instance [hA : DecidableLessOrder α] [hB : DecidableLessOrder β] : DecidableLessOrder (Array α β) :=
+instance [hA : DecidableLTOrder α] [hB : DecidableLTOrder β] : DecidableLTOrder (Array α β) :=
   { eqDec := inferInstanceAs (DecidableEq (Array α β)),
-    ltDec := inferInstanceAs (DecidableLess (Array α β))
+    ltDec := inferInstanceAs (DecidableLT (Array α β))
   }
 
 
 section Operations
-variable [DecidableLessOrder α] [DecidableLessOrder β]
+variable [DecidableLTOrder α] [DecidableLTOrder β]
 
 def select (a : Array α β) (k : α) : β :=
 match a.val.entries.lookup k with
@@ -179,16 +179,15 @@ def store (a : Array α β) (k : α) (v : β) : Array α β :=
 if h : v = a.val.default
 then
   let fm : FiniteMap α β := {a.val with entries := List.SortedMap.erase k a.val.entries};
-  have h1 : fm.entries.SortedMap from
+  have h1 : fm.entries.SortedMap :=
     List.SortedMap.erase.wellFormed k a.property.sorted;
-  have h2 : fm.entries.Forall (λ (kv : α × β) => kv.snd ≠ fm.default) from
+  have h2 : fm.entries.Forall (λ (kv : α × β) => kv.snd ≠ fm.default) :=
     List.SortedMap.erase.stillNotIn k a.property.noDefault;
   ⟨fm, ⟨h1, h2⟩⟩
 else
   let fm : FiniteMap α β := {a.val with entries := List.SortedMap.insert k v a.val.entries};
-  have h1 : fm.entries.SortedMap from
-    List.SortedMap.insert.wellFormed k v a.property.sorted;
-  have h2 : fm.entries.Forall (λ (kv : α × β) => kv.snd ≠ fm.default) from
+  have h1 : fm.entries.SortedMap := List.SortedMap.insert.wellFormed k v a.property.sorted;
+  have h2 : fm.entries.Forall (λ (kv : α × β) => kv.snd ≠ fm.default) :=
     List.SortedMap.insert.stillNotIn k h a.property.noDefault;
   ⟨fm, ⟨h1, h2⟩⟩
 
@@ -197,8 +196,8 @@ end Operations
 end Array
 
 def Array.const (α : Type u) {β : Type v} (default : β)
-  [DecidableLessOrder α]
-  [DecidableLessOrder β] : Array α β :=
+  [DecidableLTOrder α]
+  [DecidableLTOrder β] : Array α β :=
 ⟨FiniteMap.empty α default, FiniteMap.empty.wellFormed α default⟩
 
 
