deps/galois_stdlib/src/Galois/Init/Int.lean
@@ -2,13 +2,7 @@ import Galois.Init.Nat
 
 namespace Int
 
-
-
-protected
-def pow (v : Int) (n : Nat) : Int 
-  := (if Nat.bodd n ∧ v < 0 then (-1) else 1) * (Int.ofNat (v.natAbs ^ n))
-
-instance intPow : HPow Int Nat Int := ⟨Int.pow⟩
+instance intPow : Pow Int Nat := ⟨Int.pow⟩
 
 def shiftl (v : Int) (n : Nat) := v * 2 ^ n
 def shiftr (v : Int) (n : Nat) := v / 2 ^ n
